AbsSNT.v
@@ -12,8 +12,8 @@ Require Import AbsTheoryIntp.
 
 Import AbsTheorySyn AbsTheorySem.
 Import Esub GenLemmas.
-Import SN_CC_Real_old.
-Import ZF SN CCSN.
+Import SN_CC_Real.
+Import ZF SN SN_CC_Model.
 
 (*SN for the abstract theory*)
 Module Abs_SN_Theory (Msyn : TheorySyn) (Msem : TheorySem) (Mintp : TheoryIntp Msyn Msem).
