Esub.v
@@ -1,7 +1,7 @@
 Require Import GenLemmas.
 
-Import SN_CC_Real_old.
-Import ZF SN CCSN.
+Import SN_CC_Real.
+Import ZF SN SN_CC_Model.
 
 Definition esub_i := {f : val->val | Proper (eq_val ==> eq_val) f}.
 
